@prefix hmo: <https://w3id.org/hmo#> .
@prefix bot: <https://w3id.org/bot#> .
@prefix dot: <https://w3id.org/dot#> .
@prefix beo: <https://pi.pauwel.be/voc/buildingelement#> .
@prefix mat: <http://bimerr.iot.linkeddata.es/def/material-properties#> .
@prefix owl: <http://www.w3.org/2002/07/owl#> .
@prefix rdf: <http://www.w3.org/1999/02/22-rdf-syntax-ns#> .
@prefix xsd: <http://www.w3.org/2001/XMLSchema#> .
@prefix brot: <https://wisib.de/ontologie/brot#> .
@prefix foaf: <http://xmlns.com/foaf/0.1/> .
@prefix rdfs: <http://www.w3.org/2000/01/rdf-schema#> .
@prefix voaf: <http://purl.org/vocommons/voaf#> .
@prefix vann: <http://purl.org/vocab/vann/> .
@prefix schema: <http://schema.org/#> .
@prefix dcterms: <http://purl.org/dc/terms/> .

#################################################################
#    Object Properties
#################################################################

###  https://w3id.org/hmo#hasLayer
hmo:hasLayer rdf:type owl:ObjectProperty ;
                      owl:inverseOf hmo:isLayerOf ;
                          rdfs:domain hmo:MasonryWall ;
                          rdfs:range hmo:MasonryLayer ;
                          rdfs:comment  "Defines the relationship between a masonry wall and a masonry layer."@en ;
                          rdfs:label    "has layer"@en ;
						rdfs:isDefinedBy hmo: .

###  https://w3id.org/hmo#isLayerOf
hmo:isLayerOf rdf:type owl:ObjectProperty ;
                      owl:inverseOf hmo:hasLayer ;
                          rdfs:domain hmo:MasonryLayer ;
                          rdfs:range hmo:MasonryWall ;
                          rdfs:comment  "Defines the relationship between a masonry wall and a masonry layer."@en ;
                          rdfs:label    "is Layer of"@en ;
						rdfs:isDefinedBy hmo: .

###  https://w3id.org/hmo#hasHomogeneisedMechanicalProperty
hmo:hasHomogeneisedMechanicalProperty rdf:type owl:ObjectProperty ;
                      owl:inverseOf hmo:isHomogeneisedMechanicalPropertyOf ;
                          rdfs:domain hmo:MasonryWall ;
                          rdfs:range hmo:HomogeneisedMechanicalProperty ;
                          rdfs:comment  "Defines the relationship between a Masonry Wall and an Homogeneised Mechanical Property."@en ;
                          rdfs:label    "has Homogeneised Mechanical Property"@en ;
						rdfs:isDefinedBy hmo: .

###  https://w3id.org/hmo#isHomogeneisedMechanicalPropertyOf
hmo:isHomogeneisedMechanicalPropertyOf rdf:type owl:ObjectProperty ;
                      owl:inverseOf hmo:hasHomogeneisedMechanicalProperty ;
                          rdfs:domain hmo:HomogeneisedMechanicalProperty ;
                          rdfs:range hmo:MasonryWall ;
                          rdfs:comment  "Defines the relationship between an Homogeneised Mechanical Property and a Masonry Wall."@en ;
                          rdfs:label    "is Homogeneised Mechanical Property of"@en ;
						rdfs:isDefinedBy hmo: .

###  https://w3id.org/hmo#hasPattern
hmo:hasPattern rdf:type owl:ObjectProperty ;
                      owl:inverseOf hmo:isPatternOf ;
                          rdfs:domain hmo:MasonryLayer ;
                          rdfs:range hmo:Pattern ;
                          rdfs:comment  "Defines the relationship between a Masonry Layer and a Pattern."@en ;
                          rdfs:label    "has Pattern"@en ;
						rdfs:isDefinedBy hmo: .

###  https://w3id.org/hmo#isPatternOf
hmo:isPatternOf rdf:type owl:ObjectProperty ;
                      owl:inverseOf hmo:hasPattern ;
                          rdfs:domain hmo:Pattern ;
                          rdfs:range hmo:MasonryLayer ;
                          rdfs:comment  "Defines the relationship between a Pattern and a Masonry Layer."@en ;
                          rdfs:label    "is Pattern of"@en ;
						rdfs:isDefinedBy hmo: .

###  https://w3id.org/hmo#hasPatternEntity
hmo:hasPatternEntity rdf:type owl:ObjectProperty ;
                      owl:inverseOf hmo:isPatternEntityOf ;
                          rdfs:domain hmo:Pattern ;
                          rdfs:range hmo:PatternEntity ;
                          rdfs:comment  "Defines the relationship between a Pattern and a PatternEntity."@en ;
                          rdfs:label    "has PatternEntity"@en ;
						rdfs:isDefinedBy hmo: .

###  https://w3id.org/hmo#isPatternEntityOf
hmo:isPatternEntityOf rdf:type owl:ObjectProperty ;
                      owl:inverseOf hmo:hasPatternEntity ;
                          rdfs:domain hmo:PatternEntity ;
                          rdfs:range hmo:Pattern ;
                          rdfs:comment  "Defines the relationship between a PatternEntity and a Pattern."@en ;
                          rdfs:label    "is Pattern Entity of"@en ;
						rdfs:isDefinedBy hmo: .

###  https://w3id.org/hmo#hasInterfaceElements
hmo:hasInterfaceElements rdf:type owl:ObjectProperty ;
                      owl:inverseOf hmo:areInterfaceElementsOf ;
                          rdfs:domain hmo:Units ;
                          rdfs:range hmo:Joints ;
                          rdfs:comment  "Defines the relationship between Units and a Joints in a Pattern."@en ;
                          rdfs:label    "has Interface Elements"@en ;
						rdfs:isDefinedBy hmo: .

###  https://w3id.org/hmo#areInterfaceElementsOf
hmo:areInterfaceElementsOf rdf:type owl:ObjectProperty ;
                      owl:inverseOf hmo:hasInterfaceElements ;
                          rdfs:domain hmo:Joints ;
                          rdfs:range hmo:Units ;
                          rdfs:comment  "Defines the relationship between Joints and Units in a Pattern."@en ;
                          rdfs:label    "are Interface Elements of"@en ;
						rdfs:isDefinedBy hmo: .

#################################################################
#    Data properties
#################################################################

###  https://w3id.org/hmo#heigthHasMinimumValue
hmo:heigthMinimumValue rdf:type owl:DatatypeProperty ;
                          rdfs:domain hmo:Units ;
                          rdfs:range xsd:float ;
                          rdfs:comment  "Defines the minimum value of the height of the units in the pattern. "@en ;
                          rdfs:label    "Height Has Minimum Value"@en ;
						rdfs:isDefinedBy hmo: .

###  https://w3id.org/hmo#heightHasMaximumValue
hmo:heightMaximumValue rdf:type owl:DatatypeProperty ;
                          rdfs:domain hmo:Units ;
                          rdfs:range xsd:float ;
                          rdfs:comment  "Defines the maximum value of the height of the units in the pattern. "@en ;
                          rdfs:label    "Height Has Maximum Value"@en ;
						rdfs:isDefinedBy hmo: .

###  https://w3id.org/hmo#lengthHasMinimumValue
hmo:lengthMinimumValue rdf:type owl:DatatypeProperty ;
                          rdfs:domain hmo:Units ;
                          rdfs:range xsd:float ;
                          rdfs:comment  "Defines the minimum value of the length of the units in the pattern. "@en ;
                          rdfs:label    "Length Has Minimum Value"@en ;
						rdfs:isDefinedBy hmo: .

###  https://w3id.org/hmo#lengthHasMaximumValue
hmo:lengthMaximumValue rdf:type owl:DatatypeProperty ;
                          rdfs:domain hmo:Units ;
                          rdfs:range xsd:float ;
                          rdfs:comment  "Defines the maximum value of the length of the units in the pattern. "@en ;
                          rdfs:label    "Length Has Maximum Value"@en ;
						rdfs:isDefinedBy hmo: .

###  https://w3id.org/hmo#unitsHaveShape
hmo:unitsHaveShape rdf:type owl:DatatypeProperty ;
                          rdfs:domain hmo:Units ;
                          rdfs:range xsd:string ;
                          rdfs:comment  "Defines the average shape of the units. "@en ;
                          rdfs:label    "Units Have Shape"@en ;
						rdfs:isDefinedBy hmo: .

### Length has Shape / restrictions 
[
    rdf:type owl:Restriction ;
    owl:onProperty hmo:unitsHaveShape ;
    owl:hasValue "round"^^xsd:string 
] .

[
    rdf:type owl:Restriction ;
    owl:onProperty hmo:unitsHaveShape ;
    owl:hasValue "regular"^^xsd:string 
] .

[
    rdf:type owl:Restriction ;
    owl:onProperty hmo:unitsHaveShape ;
    owl:hasValue "mixed"^^xsd:string 
] .

#################################################################
#    Classes
#################################################################


###  https://w3id.org/hmo:MasonryWall
hmo:MasonryWall rdf:type owl:Class ;
			  rdfs:subClassOf beo:Wall ;
			  owl:disjointWith hmo:MasonryLayer ;
			  owl:disjointWith hmo:Pattern ;
			  owl:disjointWith hmo:PatternEntity ;
			  owl:disjointWith hmo:HomogeneisedMechanicalProperty ;
			  owl:disjointWith hmo:Source ;

              rdfs:comment """A wall made of masonry"""@en ;
			  rdfs:isDefinedBy hmo: ;
              rdfs:label "Masonry Wall"@en .

###  https://w3id.org/hmo:MasonryLayer
hmo:MasonryLayer rdf:type owl:Class ;
			  owl:disjointWith hmo:MasonryWall ;
			  owl:disjointWith hmo:Pattern ;
			  owl:disjointWith hmo:PatternEntity ;
			  owl:disjointWith hmo:HomogeneisedMechanicalProperty ;
			  owl:disjointWith hmo:Source ;

              rdfs:comment """A layer of a masonry wall"""@en ;
			  rdfs:isDefinedBy hmo: ;
              rdfs:label "Masonry Layer"@en .

###  https://w3id.org/hmo:Pattern
hmo:Pattern rdf:type owl:Class ;
			  owl:disjointWith hmo:MasonryWall ;
			  owl:disjointWith hmo:MasonryLayer ;
			  owl:disjointWith hmo:PatternEntity ;
			  owl:disjointWith hmo:HomogeneisedMechanicalProperty ;
			  owl:disjointWith hmo:Source ;

              rdfs:comment """A pattern in a masonry layer"""@en ;
			  rdfs:isDefinedBy hmo: ;
              rdfs:label "Pattern"@en .

###  https://w3id.org/hmo:PatternEntity
hmo:PatternEntity rdf:type owl:Class ;
			  owl:disjointWith hmo:MasonryWall ;
			  owl:disjointWith hmo:MasonryLayer ;
			  owl:disjointWith hmo:Pattern ;
			  owl:disjointWith hmo:HomogeneisedMechanicalProperty ;
			  owl:disjointWith hmo:Source ;

              rdfs:comment """A pattern entity in a pattern"""@en ;
			  rdfs:isDefinedBy hmo: ;
              rdfs:label "Pattern entity"@en .

###  https://w3id.org/hmo:Units
hmo:Units rdf:type owl:Class ;
			  rdfs:subClassOf hmo:PatternEntity ;
			  owl:disjointWith hmo:MasonryWall ;
			  owl:disjointWith hmo:MasonryLayer ;
			  owl:disjointWith hmo:Pattern ;
			  owl:disjointWith hmo:HomogeneisedMechanicalProperty ;
			  owl:disjointWith hmo:Source ;
			  owl:disjointWith hmo:Joints ;

              rdfs:comment """A unit configuration (units) in a pattern"""@en ;
			  rdfs:isDefinedBy hmo: ;
              rdfs:label "Units"@en .

###  https://w3id.org/hmo:Joints
hmo:Joints rdf:type owl:Class ;
			  rdfs:subClassOf hmo:PatternEntity ;
			  owl:disjointWith hmo:MasonryWall ;
			  owl:disjointWith hmo:MasonryLayer ;
			  owl:disjointWith hmo:Pattern ;
			  owl:disjointWith hmo:HomogeneisedMechanicalProperty ;
			  owl:disjointWith hmo:Source ;
			  owl:disjointWith hmo:Units ;

              rdfs:comment """The configuration of the joints in the pattern"""@en ;
			  rdfs:isDefinedBy hmo: ;
              rdfs:label "Joints"@en .

###  https://w3id.org/hmo:HomogeneisedMechanicalProperty
hmo:HomogeneisedMechanicalProperty rdf:type owl:Class ;
			  rdfs:subClassOf mat:Property ;
			  owl:disjointWith hmo:MasonryWall ;
			  owl:disjointWith hmo:MasonryLayer ;
			  owl:disjointWith hmo:Pattern ;
			  owl:disjointWith hmo:PatternEntity;
			  owl:disjointWith hmo:Source ;
			  owl:disjointWith hmo:Units ;

              rdfs:comment """The configuration of the joints in the pattern"""@en ;
			  rdfs:isDefinedBy hmo: ;
              rdfs:label "Joints"@en .
